proved confluence

Vanilla.v
@@ -1,4 +1,4 @@
-Require Import Coq.Arith.PeanoNat Coq.micromega.Lia.
+Require Import Coq.Arith.PeanoNat Coq.micromega.Lia Coq.Arith.Compare_dec.
 Require Import Lambda.Util.
 
 (** * De Bruijn Syntax of Terms *)
@@ -18,68 +18,142 @@ Notation "! n" := (Var n) (at level 0) : expr_scope.
 
 Open Scope expr_scope.
 
-(** Shifts free variables above a cutoff [c] using [op] (inc or dec). *)
-Fixpoint shift (op : nat -> nat) (c : nat) (e : expr) : expr :=
+(** Shifts free variables in [e] above a cutoff [c] up by [i]. *)
+Fixpoint lift (c i : nat) (e : expr) : expr :=
   match e with
-  | !n =>  ! if n <? c then n else op n
-  | λ e => λ (shift op (S c) e)
-  | e1 ⋅ e2 => (shift op c e1) ⋅ (shift op c e2)
+  | !n => ! match lt_dec n c with
+           | left _ => n
+           | right _ => n + i
+           end
+  | λ e => λ (lift (S c) i e)
+  | e1 ⋅ e2 => (lift c i e1) ⋅ (lift c i e2)
   end.
 (**[]*)
 
-Definition shift_up : expr -> expr := shift S 0.
-
-Definition shift_down : expr -> expr := shift pred 0.
-
-Lemma shift_c_down_up : forall e c,
-    shift pred c (shift S c e) = e.
-Proof.
-  induction e; intros; simpl; f_equal; auto.
-  destruct (n <? c) eqn:Hni;
-    simpl; try rewrite Hni; auto.
-  assert (H: S n <? c = false).
-  { rewrite Nat.ltb_ge in *; lia. }
-  rewrite H; reflexivity.
-Qed.
-
-Lemma shift_down_up : forall e,
-    shift_down (shift_up e) = e.
-Proof.
-  intros e; unfold shift_down, shift_up.
-  apply shift_c_down_up.
-Qed.
-
-(** Substitution [e{esub/m}]. *)
-Fixpoint sub (m : nat) (esub e : expr) : expr :=
+(** Substitution [e{esub/i}]. *)
+Fixpoint subst (i : nat) (esub e : expr) : expr :=
   match e with
-  | !n => if m =? n then esub else !n
-  | λ e => λ (sub (S m) (shift_up esub) e)
-  | e1 ⋅ e2 => (sub m esub e1) ⋅ (sub m esub e2)
+  | !n => match lt_eq_lt_dec i n with
+         | inleft (left _) => ! (pred n)
+         | inleft (right _) => lift 0 i esub
+         | inright _ => !n
+         end
+  | λ e => λ (subst (S i) esub e)
+  | e1 ⋅ e2 => (subst i esub e1) ⋅ (subst i esub e2)
   end.
 (**[]*)
 
-(** Beta-reduction [(λx.e1) e2 -> e1{e2/x}]. *)
-Definition beta_reduce (e1 e2 : expr) : expr :=
-  shift_down (sub 0 (shift_up e2) e1).
+Ltac compare_destruct :=
+  match goal with
+  | |- context [lt_dec ?a ?b]
+    => destruct (lt_dec a b) as [? | ?] eqn:?
+  | |- context [lt_eq_lt_dec ?a ?b]
+    => destruct (lt_eq_lt_dec a b) as [[? | ?] | ?] eqn:?
+  | |- context [match ?n with 0 => _ | S _ => _ end]
+    => destruct n as [| ?]
+  end.
 (**[]*)
 
-Lemma shift_sub : forall e es m,
-    shift pred m (sub m es (shift S m e)) = e.
-Proof.
-  induction e; intros es m; simpl; f_equal; auto.
-  - destruct (n <? m) eqn:Hnm.
-    + assert (m =? n = false).
-      { rewrite Nat.ltb_lt in Hnm.
-        rewrite Nat.eqb_neq. lia. }
-      rewrite H; simpl; rewrite Hnm; reflexivity.
-    + destruct (m =? S n) eqn:HmSn; simpl.
-      * rewrite Nat.ltb_ge in Hnm.
-        rewrite Nat.eqb_eq in HmSn; subst. lia.
-      * assert (S n <? m = false).
-        { rewrite Nat.ltb_ge in *.
-          rewrite Nat.eqb_neq in *. lia. }
-        rewrite H; reflexivity.
-Qed.
+Ltac compare_destruct_star := repeat (compare_destruct; simpl).
+
+Ltac clean_compare := compare_destruct_star; try lia; auto.
+
+Section FrenchLemmas.
+  (** The confluence proof reqiured
+      evidence of some properties of
+      shifting of de Bruijn indices.
+      What these properties were was
+      elusive to me, so I have looked
+      to the work of a wise French person,
+      who formalized the Calculus of Constructions in Coq.
+      [http://www.lix.polytechnique.fr/~barras/CoqInCoq/Termes.html] *)
+
+  Lemma lift0 : forall e k, lift k 0 e = e.
+  Proof.
+    induction e; intros; simpl;
+      clean_compare; f_equal; auto 1.
+  Qed.
+
+  Lemma simpl_lift : forall e n p k i,
+      i <= k + n -> k <= i ->
+      lift i p (lift k n e) = lift k (p + n) e.
+  Proof.
+    induction e; intros; simpl;
+      clean_compare; f_equal; auto 2; try lia.
+    apply IHe; lia.
+  Qed.
+
+  Local Hint Extern 0 => rewrite simpl_lift by lia; reflexivity : core.
+
+  Lemma permute_lift : forall e n k p i,
+      i <= k -> lift i p (lift k n e) = lift (p + k) n (lift i p e).
+  Proof.
+    induction e; intros; simpl;
+      clean_compare; f_equal; auto 2; try lia.
+    rewrite IHe by lia. f_equal; lia.
+  Qed.
+
+  Local Hint Extern 0 => rewrite permute_lift by lia; reflexivity : core.
+  
+  Lemma simpl_subst : forall M N n p k,
+      p <= n + k -> k <= p ->
+      subst p N (lift k (S n) M) = lift k n M.
+  Proof.
+    induction M; intros; simpl;
+      clean_compare; f_equal; auto 2; try lia.
+    apply IHM; lia.
+  Qed.
+
+  Local Hint Extern 0 => rewrite simpl_subst by lia; reflexivity : core.
+  
+  Lemma commute_lift_subst : forall M N n p k,
+      k <= p ->
+      lift k n (subst p N M) = subst (n + p) N (lift k n M).
+  Proof.
+    induction M; intros; simpl;
+      clean_compare;
+      try (f_equal; auto 2; lia).
+    f_equal; rewrite IHM by lia.
+    f_equal; lia.
+  Qed.
+
+  Local Hint Extern 0 => rewrite commute_lift_subst by lia; reflexivity : core.
+
+  Lemma distr_lift_subst : forall M N n p k,
+      lift (p + k) n (subst p N M) = subst p (lift k n N) (lift (S (p + k)) n M).
+  Proof.
+    induction M; intros; simpl;
+      clean_compare;
+      try (f_equal; auto 2; lia).
+    f_equal; rewrite <- IHM; f_equal; lia.
+  Qed.
+
+  Lemma distr_lift_subst0 : forall M N n k,
+      lift k n (subst 0 N M) = subst 0 (lift k n N) (lift (S k) n M).
+  Proof.
+    intros. replace k with (0 + k) at 1 by lia.
+    replace k with (0 + k) at 3 by lia.
+    apply distr_lift_subst.
+  Qed.
+  
+  Lemma distr_sub : forall M N P n p,
+      subst (p + n) P (subst p N M) =
+      subst p (subst n P N) (subst (S (p + n)) P M).
+  Proof.
+    induction M; intros; simpl;
+      clean_compare; try (f_equal; auto 2; lia).
+    f_equal; rewrite <- IHM; f_equal; lia.
+  Qed.
+
+  Lemma distr_sub0 : forall M N P n,
+      subst n P (subst 0 N M) =
+      subst 0 (subst n P N) (subst (S n) P M).
+  Proof.
+    intros. replace n with (0 + n) at 1 by lia.
+    replace n with (0 + n) at 3 by lia.
+    apply distr_sub.
+  Qed.
+End FrenchLemmas.
 
 (** * Reduction Strategies *)
 
@@ -88,7 +162,7 @@ Reserved Notation "e1 '-->' e2" (at level 40).
 
 Inductive step : expr -> expr -> Prop :=
 | step_beta e1 e2 :
-    (λ e1) ⋅ e2 -->  beta_reduce e1 e2
+    (λ e1) ⋅ e2 -->  subst 0 e2 e1
 | step_lambda e e' :
     e -->  e' ->
     λ e -->  λ e'
@@ -101,27 +175,48 @@ Inductive step : expr -> expr -> Prop :=
 where "e1 '-->' e2" := (step e1 e2).
 (**[]*)
 
+Inductive is_lambda : expr -> Prop :=
+| IsLambda e : is_lambda (λ e).
+(**[]*)
+
+Ltac not_is_lambda_lambda :=
+  match goal with
+  | H: ~ is_lambda (λ _)
+    |- _ => exfalso; apply H; constructor
+  end.
+(**[]*)
+
 (** No beta-reduxes. *)
 Inductive normal_form : expr -> Prop :=
 | nf_var n :
     normal_form !n
-| nf_app n e :
-    normal_form e ->
-    normal_form (!n ⋅ e)
+| nf_app e1 e2 :
+    ~ is_lambda e1 ->
+    normal_form e1 ->
+    normal_form e2 ->
+    normal_form (e1 ⋅ e2)
 | nf_lam e :
     normal_form e ->
     normal_form (λ e).
 (**[]*)
 
 Section NormalForm.
+  Local Hint Extern 0 => not_is_lambda_lambda : core.
+  Hint Constructors is_lambda : core.
+
+  Ltac contra_step :=
+    match goal with
+    | H: ?e -->  _, IH : (forall _, ~ ?e -->  _)
+      |- _ => apply IH in H; contradiction
+    end.
+
+  Hint Extern 0 => contra_step : core.
+
   Theorem normal_form_step : forall e e',
     normal_form e -> ~ e -->  e'.
   Proof.
     intros e e' HN; generalize dependent e';
-      induction HN; intros ? H'; inv H'.
-    - inv H2.
-    - apply IHHN in H2; contradiction.
-    - apply IHHN in H0; contradiction.
+      induction HN; intros ? H'; inv H'; auto 2.
   Qed.
 End NormalForm.
 
@@ -132,76 +227,78 @@ Definition halts (e e' : expr) : Prop :=
   e -->* e' /\ normal_form e'.
 
 Section Confluence.
-  Local Hint Constructors step : core.    
+  Local Hint Constructors step : core.
+  Local Hint Constructors refl_trans_closure : core.
   Local Hint Resolve inject_trans_closure : core.
-  Local Hint Resolve refl_closure : core.
 
   Lemma reduce_lambda : forall e e',
       e -->* e' -> λ e -->* λ e'.
-  Proof.
-    intros e e' H; induction H; auto 1.
-    transitivity (λ a2); auto 3.
-  Qed.
+  Proof. intros e e' H; induction H; eauto 3. Qed.
 
   Lemma reduce_app_l : forall e1 e1' e2,
       e1 -->* e1' -> e1 ⋅ e2 -->* e1' ⋅ e2.
-  Proof.
-    intros e1 e1' e2 H; induction H; auto 1.
-    transitivity (a2 ⋅ e2); auto 3.
-  Qed.
+  Proof. intros e1 e1' e2 H; induction H; eauto 3. Qed.
 
   Lemma reduce_app_r : forall e1 e2 e2',
       e2 -->* e2' -> e1 ⋅ e2 -->* e1 ⋅ e2'.
-  Proof.
-    intros e1 e2 e2' H; induction H; auto 1.
-    transitivity (e1 ⋅ a2); auto 3.
-  Qed.
+  Proof. intros e1 e2 e2' H; induction H; eauto 3. Qed.
 
   Local Hint Resolve reduce_lambda : core.
   Local Hint Resolve reduce_app_l : core.
   Local Hint Resolve reduce_app_r : core.
+  
+  Lemma reduce_app : forall e1 e1' e2 e2',
+      e1 -->* e1' -> e2 -->* e2' -> e1 ⋅ e2 -->* e1' ⋅ e2'.
+  Proof.
+    intros ? ? ? ? H1 H2; inv H1; inv H2; eauto 3.
+    transitivity (e1' ⋅ e2); eauto 3.
+  Qed.
 
-  Conjecture beta_reduce_inner_l : forall e1 e1' e2,
-      e1 -->  e1' -> beta_reduce e1 e2 -->* beta_reduce e1' e2.
+  Local Hint Resolve reduce_app : core.
+  
+  Lemma sub_right_step : forall er er' el c,
+      er -->  er' -> subst c el er -->  subst c el er'.
+  Proof.
+    intros ? ? el c Her;
+      generalize dependent c;
+      generalize dependent el;
+      induction Her; intros; simpl; auto 2.
+    rewrite distr_sub0; auto 1.
+  Qed.
 
-  Conjecture beta_reduce_inner_r : forall e1 e2 e2',
-      e2 -->  e2' -> beta_reduce e1 e2 -->* beta_reduce e1 e2'.
+  Lemma lift_step : forall e e' c i,
+      e -->  e' -> lift c i e -->  lift c i e'.
+  Proof.
+    intros ? ? c i He;
+      generalize dependent i;
+      generalize dependent c;
+      induction He; intros; simpl; clean_compare.
+    rewrite distr_lift_subst0; auto 1.
+  Qed.
+
+  Local Hint Resolve lift_step : core.
+  
+  Lemma sub_left_step : forall er el el' c,
+      el -->  el' -> subst c el er -->* subst c el' er.
+  Proof. induction er; intros; simpl; clean_compare. Qed.
+
+  Local Hint Resolve sub_right_step : core.
+  Local Hint Resolve sub_left_step : core.
   
   Theorem confluence : forall e e1 e2,
       e -->  e1 -> e -->  e2 -> exists e', e1 -->* e' /\ e2 -->* e'.
   Proof.
     intros ? ? e2 H1;
       generalize dependent e2;
-      induction H1; intros ? H2; inv H2; eauto 3.
-    - inv H3; exists (beta_reduce e' e2); split; auto.
-      apply beta_reduce_inner_l; assumption.
-    - exists (beta_reduce e1 e2'); split; auto.
-      apply beta_reduce_inner_r; assumption.
-    - pose proof IHstep _ H0 as [? [? ?]]; eauto.
+      induction H1; intros ? H2; inv H2; eauto 7.
+    - inv H3; eauto 6.
+    - pose proof IHstep _ H0 as [? [? ?]]; eauto 5.
     - inversion H1; subst.
-      pose proof IHstep _ H1 as [? [? ?]]; clear IHstep.
-      exists (beta_reduce e' e2); split; auto.
-      apply beta_reduce_inner_l; assumption.
-    - pose proof IHstep _ H4 as [? [? ?]]; eauto.
-    - clear IHstep. exists (e1' ⋅ e2'); split; eauto.
-    - clear IHstep. exists (beta_reduce e3 e2'); split; auto.
-      apply beta_reduce_inner_r; assumption.
-    - clear IHstep. exists (e1' ⋅ e2'); split; eauto.
-    - pose proof IHstep _ H4 as [? [? ?]]; eauto.
+      pose proof IHstep _ H1 as [? [? ?]];
+        clear IHstep; eauto 6.
+    - pose proof IHstep _ H4 as [? [? ?]]; eauto 5.
+    - pose proof IHstep _ H4 as [? [? ?]]; eauto 5.
   Qed.
-
-  Local Hint Resolve confluence : core.
-  Local Hint Constructors refl_trans_closure : core.
-
-  Corollary confluence_star :  forall e e1 e2,
-      e -->* e1 -> e -->* e2 -> exists e', e1 -->* e' /\ e2 -->* e'.
-  Proof.
-    (*intros ? ? ? He1 He2; inv He1; inv He2; eauto.*)
-    (*intros e e1 e2 He1; generalize dependent e2;
-      induction He1; intros ? He2; inv He2; eauto.
-    apply IHHe1.
-    pose proof IHHe1 _ He1 as [e' [He1' He2']].*)
-  Abort.
 End Confluence.
 
 (** Deterministic reduction. *)
@@ -209,10 +306,6 @@ End Confluence.
 Inductive shallow_value : expr -> Prop :=
 | shl_var n : shallow_value !n
 | shl_lam e : shallow_value (λ e).
-(**[]*)
-
-Inductive is_lambda : expr -> Prop :=
-| IsLambda e : is_lambda (λ e).
 (**[]*)
 
 Inductive deep_value : expr -> Prop :=
@@ -235,7 +328,7 @@ Reserved Notation "e1 '⟶' e2" (at level 40).
 Inductive cbv_reduce : expr -> expr -> Prop :=
 | cbv_beta e1 e2 :
     shallow_value e2 ->
-    (λ e1) ⋅ e2 ⟶  beta_reduce e1 e2
+    (λ e1) ⋅ e2 ⟶  subst 0 e2 e1
 | cbv_app_r e1 e2 e2' :
     shallow_value e1 ->
     e2 ⟶  e2' ->
@@ -251,7 +344,7 @@ Reserved Notation "e1 '==>' e2" (at level 40).
 
 Inductive cbn_reduce : expr -> expr -> Prop :=
 | cbn_beta e1 e2 :
-    (λ e1) ⋅ e2 ==>  beta_reduce e1 e2
+    (λ e1) ⋅ e2 ==>  subst 0 e2 e1
 | cbn_app_l e1 e1' e2 :
     e1 ==>  e1' ->
     e1 ⋅ e2 ==>  e1' ⋅ e2
@@ -263,13 +356,15 @@ Reserved Notation "e1 '>->' e2" (at level 40).
 
 Inductive normal_reduce : expr -> expr -> Prop :=
 | normal_beta e1 e2 :
-    (λ e1) ⋅ e2 >-> beta_reduce e1 e2
+    (λ e1) ⋅ e2 >-> subst 0 e2 e1
 | normal_lambda e e' :
     e >-> e' ->
     λ e >-> λ e'
-| normal_app_r n e2 e2' :
+| normal_app_r e1 e2 e2' :
+    ~ is_lambda e1 ->
+    normal_form e1 ->
     e2 >-> e2' ->
-    !n ⋅ e2 >-> !n ⋅ e2'
+    e1 ⋅ e2 >-> e1 ⋅ e2'
 | normal_app_l e1 e1' e2 :
     ~ is_lambda e1 ->
     e1 >-> e1' ->
@@ -284,7 +379,7 @@ Inductive appl_reduce : expr -> expr -> Prop :=
 | appl_beta e1 e2 :
     deep_value e1 ->
     deep_value e2 ->
-    (λ e1) ⋅ e2 ⇢ beta_reduce e1 e2
+    (λ e1) ⋅ e2 ⇢ subst 0 e2 e1
 | appl_lambda e e' :
     e ⇢ e' ->
     λ e ⇢ λ e'
@@ -296,13 +391,6 @@ Inductive appl_reduce : expr -> expr -> Prop :=
     e1 ⇢ e1' ->
     e1 ⋅ e2 ⇢ e1' ⋅ e2
 where "e1 '⇢' e2" := (appl_reduce e1 e2).
-(**[]*)
-
-Ltac not_is_lambda_lambda :=
-  match goal with
-  | H: ~ is_lambda (λ _)
-    |- _ => exfalso; apply H; constructor
-  end.
 (**[]*)
 
 Ltac cbv_step_lambda :=
@@ -352,6 +440,17 @@ Section Deep.
   Qed.
 End Deep.
 
+Section NormalFormReduce.
+  Local Hint Constructors normal_form : core.
+  Local Hint Extern 0 => not_is_lambda_lambda : core.
+
+  Lemma normal_form_reduce : forall e e',
+      e >-> e' -> ~ normal_form e.
+  Proof.
+    intros ? ? He Hnf; induction He; inv Hnf; auto 2.
+  Qed.
+End NormalFormReduce.
+
 Ltac contra_cbv_value :=
   match goal with
   | H: ?e ⟶  _, Hv: shallow_value ?e
@@ -375,8 +474,8 @@ Ltac contra_cbn_value :=
 
 Ltac contra_normal_value :=
   match goal with
-  | H: ?e >-> _, Hv: deep_value ?e
-    |- _ => apply normal_reduce_value in H; contradiction
+  | H: ?e >-> _, Hv: normal_form ?e
+    |- _ => apply normal_form_reduce in H; contradiction
   end.
 (**[]*)
 
@@ -400,6 +499,7 @@ Section Determinism.
   
   Section NORMAL.
     Local Hint Extern 0 => normal_step_app_var : core.
+    Local Hint Extern 0 => contra_normal_value : core.
     
     Theorem normal_deterministic : deterministic normal_reduce.
     Proof. ind_det; f_equal; eauto 2. Qed.
@@ -510,7 +610,7 @@ Section Normalizing.
     intros e e' [He Hnf].
     induction He; inv Hnf; auto.
     - assert (a2 >->* !n) by auto; clear IHHe. admit.
-    - assert (a2 >->* !n ⋅ e) by auto; clear IHHe. admit.
+    - assert (a2 >->* e1 ⋅ e2) by auto; clear IHHe. admit.
     - assert (a2 >->* λ e) by auto; clear IHHe. admit.
   Abort.
 End Normalizing.
@@ -518,15 +618,19 @@ End Normalizing.
 Section Examples.
   Example omega_term : expr := λ !0 ⋅ !0.
 
+  Local Hint Unfold omega_term : core.
+  Local Hint Extern 0 => not_is_lambda_lambda : core.
+  Local Hint Constructors is_lambda : core.
+
   Example omega_does_not_halt :
     forall e, ~ halts (omega_term ⋅ omega_term) e.
   Proof.
     intros e [Ho Hnf].
     remember (omega_term ⋅ omega_term) as oo eqn:Hoo.
     induction Ho; subst.
-    - inv Hnf.
+    - inv Hnf; apply H1; constructor.
     - apply IHHo; auto; clear a3 Hnf Ho IHHo; inv H; simpl; try reflexivity.
-      + inv H3. inv H0. inv H3. inv H3.
-      + inv H3. inv H0. inv H3. inv H3.
+      + inv H3. inv H0; inv H3.
+      + inv H3. inv H0; inv H3.
   Qed.
 End Examples.
